cleanup_extra

theories/SLFExtra.v
@@ -4,6 +4,9 @@ Separation Logic Foundations
 
 Chapter: "Extra".
 
+This file provides formalization of reasoning rules expressed
+using Separation Logic triples.
+
 Author: Arthur Charguéraud.
 License: MIT.
 
@@ -30,6 +33,10 @@ Definition state : Type := heap.
 (* ####################################################### *)
 (** * Additional Hoare Triples *)
 
+(** There additional extraction rules are not needed in weakest
+    precondition style because they are subsumed by corresponding
+    rules on entailment. *)
+
 Section Hoare.
 
 Lemma hoare_hforall : forall t (A:Type) (J:A->hprop) Q,
@@ -42,10 +49,8 @@ Lemma hoare_hwand_hpure_l : forall t (P:Prop) H Q,
   hoare t H Q ->
   hoare t (\[P] \-* H) Q.
 Proof using.
-  Transparent hwand.
-  introv HP M. unfold hwand. applys hoare_hexists. intros H'.
-  rewrite hstar_comm. applys hoare_hpure. intros N.
-  applys hoare_conseq M. { hchange~ N. } { hsimpl. }
+  introv HP M Hh. lets (N&_): hwand_equiv (\[P] \-* H) \[P] H.
+  forwards~ N': N h. rewrite hstar_comm. rewrite~ hstar_hpure.
 Qed.
 
 End Hoare.
@@ -58,94 +63,7 @@ End Hoare.
 (* ******************************************************* *)
 (** ** Structural rules *)
 
-Lemma triple_conseq : forall t H' Q' H Q,
-  triple t H' Q' ->
-  H ==> H' ->
-  Q' ===> Q ->
-  triple t H Q.
-Proof using.
-  introv M MH MQ. intros HF. applys hoare_conseq M.
-  { hchanges MH. }
-  { intros x. hchanges (MQ x). }
-Qed.
-
-Lemma triple_frame : forall t H Q H',
-  triple t H Q ->
-  triple t (H \* H') (Q \*+ H').
-Proof using.
-  introv M. intros HF.
-  applys hoare_conseq (M (HF \* H')); hsimpl.
-Qed.
-
-Lemma triple_htop_post : forall t H Q,
-  triple t H (Q \*+ \Top) ->
-  triple t H Q.
-Proof using.
-  introv M. intros HF.
-  applys hoare_conseq (M HF); hsimpl.
-Qed.
-
-Lemma triple_htop_pre : forall t H Q,
-  triple t H Q ->
-  triple t (H \* \Top) Q.
-Proof using.
-  introv M. applys triple_htop_post. applys~ triple_frame.
-Qed.
-
-Lemma triple_hany_pre : forall t H H' Q,
-  triple t H Q ->
-  triple t (H \* H') Q.
-Proof using.
-  introv M. applys triple_conseq.
-  { applys* triple_htop_pre. }
-  { hsimpl. } { hsimpl. }
-Qed.
-
-Lemma triple_hany_post : forall t H H' Q,
-  triple t H (Q \*+ H') ->
-  triple t H Q.
-Proof using.
-  introv M. applys triple_htop_post.
-  applys triple_conseq M; hsimpl.
-Qed.
-
-Lemma triple_conseq_frame : forall H2 H1 Q1 t H Q,
-  triple t H1 Q1 ->
-  H ==> H1 \* H2 ->
-  Q1 \*+ H2 ===> Q ->
-  triple t H Q.
-Proof using.
-  introv M WH WQ. applys triple_conseq WH WQ.
-  applys triple_frame M.
-Qed.
-
-Lemma triple_conseq_frame_htop : forall H2 H1 Q1 t H Q,
-  triple t H1 Q1 ->
-  H ==> H1 \* H2 ->
-  Q1 \*+ H2 ===> Q \*+ \Top ->
-  triple t H Q.
-Proof using.
-  introv M WH WQ. applys triple_htop_post.
-  applys triple_conseq_frame M WH WQ.
-Qed.
-
-Lemma triple_ramified_frame : forall H1 Q1 t H Q,
-  triple t H1 Q1 ->
-  H ==> H1 \* (Q1 \--* Q) ->
-  triple t H Q.
-Proof using.
-  introv M W. applys triple_conseq_frame (Q1 \--* Q) M.
-  { applys W. } { rewrite~ <- qwand_equiv. }
-Qed.
-
-Lemma triple_ramified_frame_htop : forall H1 Q1 t H Q,
-  triple t H1 Q1 ->
-  H ==> H1 \* (Q1 \--* (Q \*+ \Top)) ->
-  triple t H Q.
-Proof using. 
-  introv M W. applys triple_conseq_frame_htop (Q1 \--* Q \*+ \Top) M.
-  { applys W. } { rewrite~ <- qwand_equiv. }
-Qed.
+(** Extraction rules *)
 
 Lemma triple_hexists : forall t (A:Type) (J:A->hprop) Q,
   (forall x, triple t (J x) Q) ->
@@ -180,6 +98,94 @@ Lemma triple_hwand_hpure_l : forall t (P:Prop) H Q,
 Proof using.
   introv HP M. intros HF. applys* hoare_conseq M.
   hsimpl. applys hwand_hpure_l_intro HP.
+Qed.
+
+(** Consequence and frame rule *)
+
+Lemma triple_conseq : forall t H' Q' H Q,
+  triple t H' Q' ->
+  H ==> H' ->
+  Q' ===> Q ->
+  triple t H Q.
+Proof using.
+  introv M MH MQ. intros HF. applys hoare_conseq M.
+  { hchanges MH. }
+  { intros x. hchanges (MQ x). }
+Qed.
+
+Lemma triple_frame : forall t H Q H',
+  triple t H Q ->
+  triple t (H \* H') (Q \*+ H').
+Proof using.
+  introv M. intros HF. applys hoare_conseq (M (HF \* H')); hsimpl.
+Qed.
+
+(** Garbage rules *)
+
+Lemma triple_htop_post : forall t H Q,
+  triple t H (Q \*+ \Top) ->
+  triple t H Q.
+Proof using.
+  introv M. intros HF. applys hoare_conseq (M HF); hsimpl.
+Qed.
+
+Lemma triple_htop_pre : forall t H Q,
+  triple t H Q ->
+  triple t (H \* \Top) Q.
+Proof using.
+  introv M. applys triple_htop_post. applys~ triple_frame.
+Qed.
+
+Lemma triple_hany_pre : forall t H H' Q,
+  triple t H Q ->
+  triple t (H \* H') Q.
+Proof using.
+  introv M. applys triple_conseq (triple_htop_pre M); hsimpl.
+Qed.
+
+Lemma triple_hany_post : forall t H H' Q,
+  triple t H (Q \*+ H') ->
+  triple t H Q.
+Proof using.
+  introv M. applys triple_htop_post. applys triple_conseq M; hsimpl.
+Qed.
+
+(** Combined and ramified rules *)
+
+Lemma triple_conseq_frame_htop : forall H2 H1 Q1 t H Q,
+  triple t H1 Q1 ->
+  H ==> H1 \* H2 ->
+  Q1 \*+ H2 ===> Q \*+ \Top ->
+  triple t H Q.
+Proof using.
+  introv M WH WQ. applys triple_htop_post. 
+  applys triple_conseq WH WQ. applys triple_frame M.
+Qed.
+
+Lemma triple_conseq_frame : forall H2 H1 Q1 t H Q,
+  triple t H1 Q1 ->
+  H ==> H1 \* H2 ->
+  Q1 \*+ H2 ===> Q ->
+  triple t H Q.
+Proof using.
+  introv M WH WQ. applys triple_conseq_frame_htop M WH. hchanges WQ.
+Qed.
+
+Lemma triple_ramified_frame_htop : forall H1 Q1 t H Q,
+  triple t H1 Q1 ->
+  H ==> H1 \* (Q1 \--* (Q \*+ \Top)) ->
+  triple t H Q.
+Proof using. 
+  introv M W. applys triple_conseq_frame_htop (Q1 \--* Q \*+ \Top) M W.
+  { rewrite~ <- qwand_equiv. }
+Qed.
+
+Lemma triple_ramified_frame : forall H1 Q1 t H Q,
+  triple t H1 Q1 ->
+  H ==> H1 \* (Q1 \--* Q) ->
+  triple t H Q.
+Proof using.
+  introv M W. applys triple_ramified_frame_htop M. hchanges W.
 Qed.
 
 
@@ -261,8 +267,7 @@ Lemma triple_add : forall n1 n2,
     \[]
     (fun r => \[r = val_int (n1 + n2)]).
 Proof using.
-  intros. intros H'. applys hoare_conseq. 
-  { applys hoare_add. } { hsimpl. } { hsimpl. auto. }
+  intros. intros H'. applys hoare_conseq hoare_add; hsimpl~.
 Qed.
 
 Lemma triple_ref : forall v,
@@ -290,10 +295,36 @@ Proof using.
 Qed.
 
 
-
-
 (* ####################################################### *)
-(* LATER
+(** Disjunction and conjunction *)
+
+
+(* ---------------------------------------------------------------------- *)
+(* ** Definition and properties of [hor] *)
+
+Definition hor (H1 H2 : hprop) : hprop :=
+  \exists (b:bool), if b then H1 else H2.
+
+Lemma hor_sym : forall H1 H2,
+  hor H1 H2 = hor H2 H1.
+Proof using.
+  intros. unfold hor. applys himpl_antisym.
+  { applys himpl_hexists_l. intros b.
+    applys himpl_hexists_r (neg b). destruct* b. }
+  { applys himpl_hexists_l. intros b.
+    applys himpl_hexists_r (neg b). destruct* b. }
+Qed.
+
+(* TODO: what is the [himpl_hor_l] rule,
+   appart from unfolding the above definition of [hor]? *)
+
+Lemma himpl_hor_r_r : forall H1 H2,
+  H1 ==> hor H1 H2.
+Proof using. intros. unfolds hor. exists* true. Qed.
+
+Lemma himpl_hor_r_l : forall H1 H2,
+  H2 ==> hor H1 H2.
+Proof using. intros. unfolds hor. exists* false. Qed.
 
 Lemma triple_hor : forall t H1 H2 Q,
   triple t H1 Q ->
@@ -304,18 +335,47 @@ Proof using.
   intros b. destruct* b.
 Qed.
 
+
+(* ---------------------------------------------------------------------- *)
+(* ** Definition and properties of [hand] *)
+
+Definition hand (H1 H2 : hprop) : hprop :=
+  \forall (b:bool), if b then H1 else H2.
+
+Lemma hand_sym : forall H1 H2,
+  hand H1 H2 = hand H2 H1.
+Proof using.
+  intros. unfold hand. applys himpl_antisym.
+  { applys himpl_hforall_r. intros b.
+    applys himpl_hforall_l (neg b). destruct* b. }
+  { applys himpl_hforall_r. intros b.
+    applys himpl_hforall_l (neg b). destruct* b. }
+Qed.
+
+Lemma himpl_hand_l_r : forall H1 H2,
+  hand H1 H2 ==> H1.
+Proof using. intros. unfolds hand. applys* himpl_hforall_l true. Qed.
+
+Lemma himpl_hand_l_l : forall H1 H2,
+  hand H1 H2 ==> H2.
+Proof using. intros. unfolds hand. applys* himpl_hforall_l false. Qed.
+
+Lemma himpl_hand_r : forall H1 H2 H3,
+  H1 ==> H2 ->
+  H1 ==> H3 ->
+  H1 ==> hand H2 H3.
+Proof using.
+  introv M1 M2. unfold hand. applys himpl_hforall_r. intros b. case_if*.
+Qed.
+
 Lemma triple_hand_l : forall t H1 H2 Q,
   triple t H1 Q ->
   triple t (hand H1 H2) Q.
-Proof using.
-  introv M1. unfold hand. applys triple_hforall. exists* true.
-Qed.
+Proof using. introv M1. unfold hand. applys~ triple_hforall true. Qed.
 
 Lemma triple_hand_r : forall t H1 H2 Q,
   triple t H2 Q ->
   triple t (hand H1 H2) Q.
-Proof using.
-  introv M1. unfold hand. applys triple_hforall. exists* false.
-Qed.
+Proof using. introv M1. unfold hand. applys~ triple_hforall false. Qed.
 
-*)
+
